sha3_cmp_impl_soundness.v
@@ -28,6 +28,10 @@ Require Import FORVES.symbolic_state_eval.
 Import SymbolicStateEval.
 
 
+Require Import FORVES.symbolic_state_eval_facts.
+Import SymbolicStateEvalFacts.
+
+
 Require Import FORVES.valid_symbolic_state.
 Import ValidSymbolicState.
 
@@ -43,6 +47,12 @@ Import SHA3CmpImpl.
 Require Import FORVES.eval_common.
 Import EvalCommon.
 
+Require Import FORVES.memory_cmp_impl_soundness.
+Import MemoryCmpImplSoundness.
+
+Require Import FORVES.concrete_interpreter.
+Import ConcreteInterpreter.
+
 Module SHA3CmpImplSoundness.
 
 
@@ -56,10 +66,1055 @@ Module SHA3CmpImplSoundness.
     intros.
     discriminate.
   Qed.
+
+
+  Lemma N_n_Sm_le_p_imp_m_lt_p:
+    forall (m: nat) (n p: N),
+      (n + N.of_nat (S m) <= p -> n<p)%N.
+  Proof.
+    intros m n p H.
+    (* *)
+    assert(H0: (N.of_nat (S m) > 0)%N). rewrite N.gt_lt_iff. Search N.to_nat. apply Nlt_in. simpl. intuition.
+    (* *)
+
+    (* *)
+    assert (H1: (n < n + N.of_nat (S m))%N). rewrite N.gt_lt_iff in H0. pose proof (N.lt_add_pos_r (N.of_nat (S m)) n H0) as H2. apply H2.
+    (* *)
+
+    pose proof (N.lt_le_trans n (n + N.of_nat (S m)) p H1 H) as H2.
+    apply H2.
+  Qed.
+  
+  Lemma mload_''_remove_first_update:
+    forall (size: nat) (offset0 offset1: N) v mem,
+    (offset0 < offset1)%N ->
+       mload'' (fun offset : N => if (offset =? offset0)%N then v else mem offset) offset1 size =
+         mload'' mem offset1 size.
+  Proof.
+    induction size as [|size' IHsize'].
+    + intros offset0 offset1 v mem H_b.
+      simpl.
+      reflexivity.
+    + intros offset0 offset1 v mem H_b.
+      unfold mload''.
+      fold mload''.
+      pose proof (@or_introl (offset0 < offset1)%N (offset1 < offset0)%N H_b) as H_b_ext.
+      apply N.lt_gt_cases in H_b_ext.
+      rewrite <- N.eqb_neq in H_b_ext.
+      rewrite N.eqb_sym.
+      rewrite H_b_ext.
+      apply N.lt_lt_succ_r in H_b as H_b2.
+      rewrite <- N.add_1_r in H_b2.     
+      pose proof (IHsize' offset0 (offset1+1)%N v mem H_b2) as IHsize'_0.
+      rewrite  IHsize'_0.
+      reflexivity.
+  Qed.
+
+  Lemma mload''_mstore'_out_of_slot'_1:
+    forall (sz: nat) mem (offset offset': N) (size: nat) (value: word (sz*8)),
+    (offset' + (N.of_nat sz) <= offset )%N ->
+    exists v,
+      mload'' mem offset size = v /\
+      mload'' (mstore' mem value offset') offset size = v.
+  Proof.
+    induction sz as [|sz' IHsz'].
+    + intros mem offset offset' size value H_b.
+      simpl.
+      exists (mload'' mem offset size).
+      split; reflexivity.
+    + intros mem offset offset' size value H_b.
+      simpl.
+
+      assert (H_offset'_lt_offsset: (offset' < offset)%N). pose proof (N_n_Sm_le_p_imp_m_lt_p sz' offset' offset H_b) as H0. apply H0.
+      
+      
+      pose proof (mload_''_remove_first_update size offset' offset (split1_byte value) (mstore' mem (split2_byte value) (offset' + 1)) H_offset'_lt_offsset) as H_mload_''_remove_first_update.
+      rewrite H_mload_''_remove_first_update.
+      
+      assert( H_bb : (offset' + 1 + N.of_nat sz' <= offset)%N). rewrite Nat2N.inj_succ in H_b. simpl in H_b. rewrite <- N.add_1_l in H_b. rewrite N.add_assoc in H_b. apply H_b.
+      
+      pose proof (IHsz' mem offset (offset' + 1)%N size (split2_byte value) H_bb) as IHsz'_0.
+      destruct IHsz'_0 as [v' IHsz'_0].
+      exists v'.
+      apply IHsz'_0.
+Qed.
+
+  
+    Lemma mem'_mstore'_out_of_slot'_1:
+    forall (sz: nat) mem (offset offset': N) (value: word (sz*8)),
+      (offset < offset')%N ->
+      exists v,
+        mem offset = v /\
+          (mstore' mem value offset') offset = v.
+  Proof.
+    induction sz as [|sz' IHsz'].
+    + intros mem offset offset' value H_b.
+      simpl.
+      exists (mem offset).
+      split; reflexivity.
+    + intros mem offset offset' value H_b.
+      simpl.
+
+      (* *)
+      assert(H_offset_neq_offset': (offset =? offset' = false)%N).
+        pose proof (@or_introl (offset < offset')%N (offset' < offset)%N H_b) as H_b_ext.
+        apply N.lt_gt_cases in H_b_ext.
+        rewrite <- N.eqb_neq in H_b_ext.
+        apply H_b_ext.
+      (* *)
+      
+      rewrite H_offset_neq_offset'.
+      assert(H_bb: (offset < offset'+1)%N). apply N.lt_lt_add_r. apply H_b.
+      
+      pose proof (IHsz' mem offset (offset'+1)%N (split2_byte value) H_bb) as IHsz'_0.
+      destruct IHsz'_0 as [v' [IHsz'_0 IHsz'_1]].
+      rewrite IHsz'_0.
+      rewrite IHsz'_1.
+      exists v'.
+      split; reflexivity.
+Qed.
+
+  
+  Lemma mload''_mstore'_out_of_slot'_2:
+    forall (size: nat)  (sz: nat) mem (offset offset': N) (value: word (sz*8)),
+    (offset + (N.of_nat size) <= offset')%N ->
+    exists v,
+      mload'' mem offset size = v /\
+      mload'' (mstore' mem value offset') offset size = v.
+  Proof.
+    induction size as [|size' IHsize'].
+    + intros sz mem offset offset' value H_b.
+      simpl.
+      exists WO.
+      split; reflexivity.
+    + intros sz mem offset offset' value H_b.
+      unfold mload''.
+      fold mload''.
+      (* *)
+      assert(H_bb: (offset + 1 + N.of_nat size' <= offset')%N).
+        rewrite Nat2N.inj_succ in H_b. simpl in H_b. rewrite <- N.add_1_l in H_b. rewrite N.add_assoc in H_b. apply H_b.
+        (* *)
+        
+      pose proof (IHsize' sz mem (offset+1)%N offset' value H_bb) as IHsize'_0.
+      destruct IHsize'_0 as [v' [IHsize'_0 IHsize'_1]].
+      rewrite IHsize'_0.
+      rewrite IHsize'_1.
+
+      (* *)
+      assert (H_offset_lt_offsset': (offset < offset')%N). pose proof (N_n_Sm_le_p_imp_m_lt_p size' offset offset' H_b) as H0. apply H0.
+      (* *)
+      
+      pose proof (mem'_mstore'_out_of_slot'_1 sz mem offset offset' value H_offset_lt_offsset') as H_mem'_mstore'_out_of_slot'_1.
+      destruct H_mem'_mstore'_out_of_slot'_1 as [v'' [H_mem'_mstore'_out_of_slot'_1_0 H_mem'_mstore'_out_of_slot'_1_1]].
+      rewrite <- H_mem'_mstore'_out_of_slot'_1_0 in H_mem'_mstore'_out_of_slot'_1_1.
+      rewrite H_mem'_mstore'_out_of_slot'_1_1.
+      exists (Word.combine (mem offset) v').
+      split; reflexivity.
+Qed.      
+        
+                                 
+
+  Lemma remove_out_of_slot'_valid:
+    forall (min max: N) (smem smem': smemory) (maxidx : nat) (sb : sbindings) (instk_height : nat) (ops : stack_op_instr_map),
+      valid_bindings instk_height maxidx sb ops ->
+  valid_smemory instk_height maxidx smem ->
+  remove_out_of_slot' smem min max maxidx sb instk_height ops = smem' ->
+  valid_smemory instk_height maxidx smem'.
+  Proof.
+    intros min max.
+    induction smem as [|u smem'' IHsmem''].
+    + intros smem' maxidx sb instk_height ops.
+      intros H_valid_sb H_valid_smem H_remove_out_of_slot'.
+      simpl in H_remove_out_of_slot'.
+      rewrite <- H_remove_out_of_slot'.
+      simpl.
+      apply I.
+    + intros smem' maxidx sb instk_height ops.
+      intros H_valid_sb H_valid_smem H_remove_out_of_slot'.
+      unfold remove_out_of_slot' in H_remove_out_of_slot'.
+      fold remove_out_of_slot' in H_remove_out_of_slot'.
+      
+      simpl in H_valid_smem.
+      destruct H_valid_smem as [H_valid_u H_valid_smem''].
+      destruct (update_out_of_slot u min max maxidx sb instk_height ops) eqn:H_out_of_slot.
+      
+      ++ pose proof (IHsmem'' smem' maxidx sb instk_height ops  H_valid_sb H_valid_smem'' H_remove_out_of_slot') as IHsmem''_0.
+         apply IHsmem''_0.
+      ++ remember (remove_out_of_slot' smem'' min max maxidx sb instk_height ops) as smem'''.
+         pose proof (IHsmem'' smem''' maxidx sb instk_height ops  H_valid_sb H_valid_smem''  (eq_sym Heqsmem''')) as IHsmem''_0.
+         rewrite <- H_remove_out_of_slot'.
+         simpl; intuition.
+  Qed.
+  
+
+  Lemma update_out_of_slot_snd_d1_aux_0:
+    forall (n: nat) (value: word (n*8)) (offset' offset: N) (mem mem': memory),
+      (N.to_nat offset) < (N.to_nat offset') ->
+      mstore' mem value offset' = mem' ->
+        (mem offset) = (mem' offset).
+  Proof.
+    induction n as [|n' IHn'].
+    + intros value offset' offset mem mem' H_b H_mstore.
+      simpl in H_mstore.
+      rewrite H_mstore.
+      reflexivity.
+    +  intros value offset' offset mem mem' H_b H_mstore.
+       rewrite <- H_mstore.
+       simpl.
+       destruct (offset =? offset')%N eqn:E_o_o'.
+       ++ apply N.eqb_eq in E_o_o'.
+          rewrite E_o_o' in H_b.
+          intuition.
+       ++ assert(H_o: (N.to_nat offset) < (N.to_nat (offset'+1))). intuition.
+          remember (mstore' mem (split2_byte value) (offset' + 1)) as mem''.
+          apply (IHn' (split2_byte value) (offset'+1)%N offset mem mem'' H_o (eq_sym Heqmem'')).
+  Qed.
+
+
+    Lemma update_out_of_slot_snd_d1_aux_1:
+    forall size offset offset' mem v,
+      (offset+ (N.of_nat size) <= offset')%N ->
+      (mload'' (fun o : N => if (o =? offset')%N then v else mem o) offset size)
+      = mload'' mem offset size.
+  Proof.
+    induction size as [|size' IHsize'].
+    + simpl. intros. reflexivity.
+    + intros offset offset' mem v H_b.
+      simpl.
+      destruct (offset =? offset')%N eqn:E_o_o'.
+      ++ apply N.eqb_eq in E_o_o'.
+         rewrite E_o_o' in H_b.
+         intuition.
+      ++ assert(H_b1: (offset + 1 + N.of_nat size' <= offset')%N).
+         pose proof (memory_ops_solvers_impl_soundness.MemoryOpsSolversImplSoundness.N_of_nat_Sn offset size') as H0.
+         rewrite H0 in H_b.
+         apply H_b.
+         rewrite (IHsize' (offset+1)%N offset' mem v H_b1).
+         reflexivity.
+  Qed.
+
+
+  Lemma update_out_of_slot_snd_d1_aux:
+    forall (n: nat) size (value: word (n*8)) (offset' offset: N) (mem mem': memory),
+      (N.to_nat offset) + size <= (N.to_nat offset') ->
+      mstore' mem value offset' = mem' ->
+        (mload'' mem offset size) = (mload'' mem' offset size).
+  Proof.
+    induction n as [|n' IHn'].
+    + intros size value offset' offset mem mem' H_b H_mstore.
+      simpl in H_mstore.
+      rewrite H_mstore.
+      reflexivity.
+    + intros size value offset' offset mem mem' H_b H_mstore.
+      destruct size as [|size']; try reflexivity.
+      rewrite <- H_mstore.
+ 
+      simpl.
+
+      destruct (offset =? offset')%N eqn:E_o_o'.
+      ++ apply N.eqb_eq in E_o_o'.
+         rewrite E_o_o' in H_b.
+         intuition.
+      ++ remember (mstore' mem (split2_byte value) (offset' + 1)) as mem''.
+         assert(H_o1: N.to_nat offset < N.to_nat (offset' + 1)%N). intuition.
+         rewrite (update_out_of_slot_snd_d1_aux_0 n' (split2_byte value) (offset' + 1)%N offset mem mem'' H_o1 (eq_sym Heqmem'')).
+         assert(H_b1: (offset + 1 + N.of_nat size' <= offset')%N).
+         rewrite <- (memory_ops_solvers_impl_soundness.MemoryOpsSolversImplSoundness.N_of_nat_Sn offset size').
+         apply Nle_in.
+         intuition.
+         rewrite (update_out_of_slot_snd_d1_aux_1 size' (offset+1)%N offset' mem'' (split1_byte value) H_b1).
+         assert(H_o2: N.to_nat (offset + 1) + size' <= N.to_nat (offset' + 1)). intuition.
+         rewrite (IHn' size' (split2_byte value) (offset' + 1)%N (offset + 1)%N mem mem'' H_o2 (eq_sym Heqmem'')).
+         reflexivity.
+  Qed.
+
+
+  
+  Lemma update_out_of_slot_snd_d2_aux_0:
+    forall (n: nat) (value: word (n*8)) (offset' offset: N) (mem mem': memory),
+      (N.to_nat offset') + n <= (N.to_nat offset) ->
+      mstore' mem value offset' = mem' ->
+      (mem offset) = (mem' offset).
+  Proof.
+    induction n as [|n' IHn'].
+    + intros value offset' offset mem mem' H_b H_mstore.
+      simpl in H_mstore.
+      rewrite H_mstore.
+      reflexivity.
+    +  intros value offset' offset mem mem' H_b H_mstore.
+       rewrite <- H_mstore.
+       simpl.
+       destruct (offset =? offset')%N eqn:E_o_o'.
+       ++ apply N.eqb_eq in E_o_o'. intuition.
+       ++ assert(H_o: N.to_nat (offset' + 1) + n' <= N.to_nat offset). intuition.
+          remember (mstore' mem (split2_byte value) (offset' + 1)) as mem''.
+          apply (IHn' (split2_byte value) (offset'+1)%N offset mem mem'' H_o (eq_sym Heqmem'')).
+Qed.
+
+  Lemma update_out_of_slot_snd_d2_aux_1:
+    forall size offset offset' mem v,
+      (offset' < offset)%N ->
+      (mload'' (fun o : N => if (o =? offset')%N then v else mem o) offset size)
+      = mload'' mem offset size.
+  Proof.
+    induction size as [|size' IHsize'].
+    + simpl. intros. reflexivity.
+    + intros offset offset' mem v H_b.
+      simpl.
+      destruct (offset =? offset')%N eqn:E_o_o'.
+      ++ apply N.eqb_eq in E_o_o'. intuition.
+      ++ assert(H_b1: (offset' < offset+1)%N).
+         apply N.lt_lt_add_r.
+         apply H_b.         
+         rewrite (IHsize' (offset+1)%N offset' mem v H_b1).
+         reflexivity.
+Qed.
+
+  Lemma update_out_of_slot_snd_d2_aux:
+    forall (n: nat) size (value: word (n*8)) (offset' offset: N) (mem mem': memory),
+      (N.to_nat offset') + n <= (N.to_nat offset) ->
+      mstore' mem value offset' = mem' ->
+      (mload'' mem offset size) = (mload'' mem' offset size).
+  Proof.
+    induction n as [|n' IHn'].
+    + intros size value offset' offset mem mem' H_b H_mstore.
+      simpl in H_mstore.
+      rewrite H_mstore.
+      reflexivity.
+    + intros size value offset' offset mem mem' H_b H_mstore.
+      destruct size as [|size']; try reflexivity.
+      rewrite <- H_mstore.
+ 
+      simpl.
+
+      destruct (offset =? offset')%N eqn:E_o_o'.
+      ++ apply N.eqb_eq in E_o_o'.
+         rewrite E_o_o' in H_b.         
+         intuition.
+      ++ remember (mstore' mem (split2_byte value) (offset' + 1)) as mem''.
+         assert(H_o1: (N.to_nat (offset' + 1) + n' <= N.to_nat offset)). intuition.
+         rewrite (update_out_of_slot_snd_d2_aux_0 n' (split2_byte value) (offset' + 1)%N offset mem mem'' H_o1 (eq_sym Heqmem'')).
+         assert(H_b1: (offset' < offset + 1)%N).  apply Nlt_in. intuition.
+          Search (N.to_nat ?a < N.to_nat ?b).
+         rewrite (update_out_of_slot_snd_d2_aux_1 size' (offset+1)%N offset' mem'' (split1_byte value) H_b1).
+         assert(H_o2: N.to_nat (offset' + 1) + n' <= N.to_nat (offset + 1)). intuition.
+         rewrite (IHn' size' (split2_byte value) (offset' + 1)%N (offset + 1)%N mem mem'' H_o2 (eq_sym Heqmem'')).
+         reflexivity.
+Qed.
+
+  Lemma update_out_of_slot_snd_aux:
+    forall (n: nat) size (value: word (n*8)) (offset' offset: N) (mem mem': memory),
+      (N.to_nat offset) + size  <= (N.to_nat offset') \/ (N.to_nat offset') + n <= (N.to_nat offset)
+      ->
+      mstore' mem value offset' = mem' ->
+      (mload'' mem offset size) = (mload'' mem' offset size).
+  Proof.
+    intros n size value offset' offset mem mem' H_b H_mstore'.
+    destruct H_b as [H_b1 | H_b2].
+    + apply (update_out_of_slot_snd_d1_aux n size value offset' offset mem mem' H_b1 H_mstore').
+    + apply (update_out_of_slot_snd_d2_aux n size value offset' offset mem mem' H_b2 H_mstore').
+  Qed.
+  
+  Lemma update_out_of_slot_snd_1:
+    forall (min max: N) (u: memory_update sstack_val) (smem: smemory) (maxidx : nat) (sb : sbindings) (instk_height : nat) (ops : stack_op_instr_map) (stk : list EVMWord) (mem : memory) (strg : storage) (exts : externals) (mem1 mem1' : memory) (offset size : EVMWord),    
+      length stk = instk_height ->    
+      valid_bindings instk_height maxidx sb ops ->
+      valid_smemory instk_height maxidx smem ->
+      valid_smemory_update instk_height maxidx u ->
+      eval_smemory smem maxidx sb stk mem strg exts ops = Some mem1 ->
+      eval_smemory (u::smem) maxidx sb stk mem strg exts ops = Some mem1' ->
+      ((wordToN offset) >= min)%N ->
+      (((wordToN offset)+(wordToN size)) <= max)%N ->
+      update_out_of_slot u min max maxidx sb instk_height ops = true ->
+      exists v,
+        (mload' mem1 offset (wordToNat size)) = v /\
+          (mload' mem1' offset (wordToNat size)) = v.
+  Proof.
+    intros min max u smem maxidx sb instk_height ops stk mem strg exts mem1 mem1' offset size.
+    intros H_stk_len H_valid_bs H_valid_smem H_valid_u H_eval_smem H_eval_u_smem H_lb H_ub H_update_oos.
+
+    unfold eval_smemory in H_eval_smem.
+    destruct (map_option (instantiate_memory_update (fun sv : sstack_val => eval_sstack_val sv stk mem strg exts maxidx sb ops)) smem) as [updates|] eqn:E_mo_updates; try discriminate.
+    injection H_eval_smem as H_mem1.
+
+    unfold eval_smemory in H_eval_u_smem.
+    destruct (map_option (instantiate_memory_update (fun sv : sstack_val => eval_sstack_val sv stk mem strg exts maxidx sb ops)) (u::smem)) as [u_updates|] eqn:E_mo_u_updates; try discriminate.
+    injection H_eval_u_smem as H_mem1'.
+
+    pose proof (map_option_split (memory_update sstack_val) (memory_update EVMWord) (instantiate_memory_update (fun sv : sstack_val => eval_sstack_val sv stk mem strg exts maxidx sb ops)) smem u_updates u E_mo_u_updates) as E_mo_u_updates_0.
+    destruct E_mo_u_updates_0 as [uv [updates' [H_u_updates [H_uv E_mo_updates']]]].
+    rewrite E_mo_updates in E_mo_updates'.
+    injection E_mo_updates' as E_updates'.
+    rewrite <- E_updates' in H_u_updates.
+
+    rewrite H_u_updates in H_mem1'.
+    simpl in H_mem1'.
+    rewrite H_mem1 in H_mem1'.
     
+    destruct u as [uoffset uvalue|uoffset uvalue] eqn:E_u.
+    + unfold update_out_of_slot in H_update_oos.
+      destruct (follow_in_smap uoffset maxidx sb) eqn:E_follow_uoffset; try discriminate.
+      destruct f; try discriminate.
+      destruct smv; try discriminate.
+      destruct val; try discriminate.
+      simpl in H_uv.
+      unfold eval_sstack_val in H_uv at 1.
+      unfold eval_sstack_val' in H_uv.
+      fold eval_sstack_val' in H_uv.
+      rewrite E_follow_uoffset in H_uv.
+
+      simpl in H_valid_u.
+      destruct H_valid_u as [H_valid_uoffset H_valid_uvalue].
+      
+      pose proof (eval_sstack_val_succ sb instk_height uvalue stk mem strg exts maxidx ops (eq_sym H_stk_len) H_valid_uvalue H_valid_bs) as H_eval_uvalue.
+      destruct H_eval_uvalue as [uvalue_v H_eval_uvalue].
+      rewrite H_eval_uvalue in H_uv.
+      injection H_uv as H_uv.
+
+      rewrite <- H_uv in H_mem1'.
+      simpl in H_mem1'.
+      unfold mstore in H_mem1'.
+
+      unfold mload'.
+
+      apply orb_prop in H_update_oos.
+
+      assert(H_b: N.to_nat (wordToN offset) + wordToNat size <= N.to_nat (wordToN val) \/
+                    N.to_nat (wordToN val) + BytesInEVMWord <= N.to_nat (wordToN offset) ).
+
+      (* of assert *)
+      ++ destruct H_update_oos as [H_update_oos | H_update_oos].
+         +++ right.
+             rewrite N.ltb_lt in H_update_oos.
+             apply N.ge_le in H_lb.
+             pose proof (N.lt_le_trans (wordToN val + 31)%N min (wordToN offset) H_update_oos H_lb) as H0.
+             apply Nlt_out in H0.
+             apply lt_le_S in H0.
+             rewrite N2Nat.inj_add in H0.
+             rewrite <- Nat.add_succ_r in H0.
+             simpl in H0.
+             apply H0.
+         +++ left.
+             rewrite N.leb_le in H_update_oos.
+             
+             pose proof (N.le_trans (wordToN offset + wordToN size)%N max (wordToN val) H_ub H_update_oos) as H0.
+             rewrite <- wordToN_to_nat.
+             pose proof (N2Nat.inj_add (wordToN offset) (wordToN size)) as H1.
+             rewrite <- H1. 
+             intuition.
+      ++ pose proof (update_out_of_slot_snd_aux BytesInEVMWord (wordToNat size) uvalue_v (wordToN val) (wordToN offset) mem1 mem1' H_b H_mem1') as H_mload''.
+         rewrite H_mload''.
+         exists (mload'' mem1' (wordToN offset) (wordToNat size)).
+         split; try reflexivity.
+    + unfold update_out_of_slot in H_update_oos.
+      destruct (follow_in_smap uoffset maxidx sb) eqn:E_follow_uoffset; try discriminate.
+      destruct f; try discriminate.
+      destruct smv; try discriminate.
+      destruct val; try discriminate.
+      simpl in H_uv.
+      unfold eval_sstack_val in H_uv at 1.
+      unfold eval_sstack_val' in H_uv.
+      fold eval_sstack_val' in H_uv.
+      rewrite E_follow_uoffset in H_uv.
+
+      simpl in H_valid_u.
+      destruct H_valid_u as [H_valid_uoffset H_valid_uvalue].
+      
+      pose proof (eval_sstack_val_succ sb instk_height uvalue stk mem strg exts maxidx ops (eq_sym H_stk_len) H_valid_uvalue H_valid_bs) as H_eval_uvalue.
+      destruct H_eval_uvalue as [uvalue_v H_eval_uvalue].
+      rewrite H_eval_uvalue in H_uv.
+      injection H_uv as H_uv.
+
+      rewrite <- H_uv in H_mem1'.
+      simpl in H_mem1'.
+      unfold mstore in H_mem1'.
+
+      unfold mload'.
+      
+      apply orb_prop in H_update_oos.
+
+       assert(H_b: (N.to_nat (wordToN offset) + wordToNat size <= N.to_nat (wordToN val) \/ N.to_nat (wordToN val) + 1 <= N.to_nat (wordToN offset))). 
+
+      (* of assert *)
+      ++ destruct H_update_oos as [H_update_oos | H_update_oos].
+         +++ right.
+             rewrite N.ltb_lt in H_update_oos.
+             intuition.
+         +++ left.
+             rewrite N.leb_le in H_update_oos.
+             pose proof (N.le_trans (wordToN offset + wordToN size)%N max (wordToN val) H_ub H_update_oos) as H0.
+             rewrite <- wordToN_to_nat.
+             pose proof (N2Nat.inj_add (wordToN offset) (wordToN size)) as H1.
+             rewrite <- H1. 
+             intuition.
+       (*end *)
+      ++ pose proof (update_out_of_slot_snd_aux 1 (wordToNat size) (split1_byte (uvalue_v: word ((S (pred BytesInEVMWord))*8))) (wordToN val) (wordToN offset) mem1 mem1' H_b H_mem1') as H_mload''.
+      rewrite H_mload''.
+      exists (mload'' mem1' (wordToN offset) (wordToNat size)).
+      split; try reflexivity.
+  Qed.
+
+
+  Lemma eval_smemory_u_mem_0:
+    forall size offset offset' mem1 mem2 value,
+      mload'' mem1 offset size = mload'' mem2 offset size ->
+      mload'' (fun o' => if (offset' =? o')%N then value else mem1 o') offset size = mload'' (fun o' => if (offset' =? o')%N then value else mem2 o') offset size.
+  Proof.
+    induction size as [|size' IHsize'].
+    + reflexivity.
+    + intros offset offset' mem1 mem2 value H_mload''_mem1_mem2.
+      simpl.
+      
+      simpl in H_mload''_mem1_mem2.
+      pose proof (@combine_inj 8 (size'*8) (mem1 offset) (mload'' mem1 (offset + 1) size') (mem2 offset) (mload'' mem2 (offset + 1) size') H_mload''_mem1_mem2 ) as H_combine_inj.
+      destruct H_combine_inj as [H_combine_inj_1 H_combine_inj_2].
+      
+      destruct (offset' =? offset)%N eqn:E_o_offse.
+      ++ pose proof (IHsize' (offset+1)%N offset' mem1 mem2 value H_combine_inj_2) as IHsize'_0.
+         rewrite IHsize'_0.
+         reflexivity.
+      ++ pose proof (IHsize' (offset+1)%N offset' mem1 mem2 value H_combine_inj_2) as IHsize'_0.
+         rewrite IHsize'_0.
+         rewrite H_combine_inj_1.
+         reflexivity.
+  Qed.
+  
+  Lemma eval_smemory_u_mem_1:
+    forall n size offset offset' mem1 mem2 mem1' mem2' (value : word (n*8)) ,
+      mload'' mem1 offset (S size) = mload'' mem2 offset (S size) ->
+      mstore' mem1 value offset' = mem1' ->
+      mstore' mem2 value offset' = mem2' ->
+      mem1' offset = mem2' offset.
+  Proof.
+    induction n as [|n' IHn'].
+    + intros size offset offset' mem1 mem2 mem1' mem2' value H_mload'' H_mstore'_mem1 H_mstore'_mem2.
+      rewrite <- H_mstore'_mem1.
+      rewrite <- H_mstore'_mem2.
+      simpl.
+      pose proof (@combine_inj 8 (size*8) (mem1 offset) (mload'' mem1 (offset + 1) size) (mem2 offset) (mload'' mem2 (offset + 1) size) H_mload'' ) as H_combine_inj.
+      destruct H_combine_inj as [H_combine_inj_1 H_combine_inj_2].
+      apply H_combine_inj_1.
+    + intros size offset offset' mem1 mem2 mem1' mem2' value H_mload'' H_mstore'_mem1 H_mstore'_mem2.
+      rewrite <- H_mstore'_mem1.
+      rewrite <- H_mstore'_mem2.
+      simpl.
+      destruct (offset =? offset')%N; try reflexivity.
+      remember (mstore' mem1 (split2_byte value) (offset' + 1)) as mem1''.
+      remember (mstore' mem2 (split2_byte value) (offset' + 1)) as mem2''.
+      pose proof (IHn' size offset (offset'+1)%N mem1 mem2 mem1'' mem2'' (split2_byte value) H_mload'' (eq_sym Heqmem1'') (eq_sym Heqmem2'')) as IHn'_0.
+      apply IHn'_0.
+  Qed.
+  
+  Lemma eval_smemory_u_mem_2:
+    forall size n offset offset' mem1 mem2 mem1' mem2' (value : word (n*8)) ,
+      mload'' mem1 offset size = mload'' mem2 offset size ->
+      mstore' mem1 value offset' = mem1' ->
+      mstore' mem2 value offset' = mem2' ->
+      mload'' mem1' offset size = mload'' mem2' offset size.
+  Proof. 
+    induction size as [|size' IHsize'].
+    + intros n offset offset' mem1 mem2 mem1' mem2' value H_mload''_mem1_mem2 H_mstore'_mem1 H_mstore'_mem2.
+      simpl.
+      reflexivity. 
+    + induction n as [|n' IHn'].
+      ++ intros offset offset' mem1 mem2 mem1' mem2' value H_mload''_mem1_mem2 H_mstore'_mem1 H_mstore'_mem2. 
+         simpl in H_mload''_mem1_mem2.
+         pose proof (@combine_inj 8 (size'*8) (mem1 offset) (mload'' mem1 (offset + 1) size') (mem2 offset) (mload'' mem2 (offset + 1) size') H_mload''_mem1_mem2 ) as H_combine_inj.
+         destruct H_combine_inj as [H_combine_inj_1 H_combine_inj_2].
+         simpl.
+         pose proof (IHsize' 0 (offset + 1)%N offset' mem1 mem2 mem1' mem2' value H_combine_inj_2 H_mstore'_mem1 H_mstore'_mem2) as IHsize'_0.
+         rewrite IHsize'_0.
+         (**)
+         assert (H_mem1'_mem2': mem1' offset = mem2' offset).
+         rewrite <- H_mstore'_mem1.
+         rewrite <- H_mstore'_mem2.
+         simpl.
+         apply H_combine_inj_1.
+         rewrite H_mem1'_mem2'.
+         reflexivity.
+      ++ intros offset offset' mem1 mem2 mem1' mem2' value H_mload''_mem1_mem2 H_mstore'_mem1 H_mstore'_mem2.
+         assert(H_mload''_mem1_mem2_0 := H_mload''_mem1_mem2).
+         simpl in H_mload''_mem1_mem2.
+         pose proof (@combine_inj 8 (size'*8) (mem1 offset) (mload'' mem1 (offset + 1) size') (mem2 offset) (mload'' mem2 (offset + 1) size') H_mload''_mem1_mem2 ) as H_combine_inj.
+         destruct H_combine_inj as [H_combine_inj_1 H_combine_inj_2].
+         simpl.
+         pose proof (IHsize' (S n') (offset + 1)%N offset' mem1 mem2 mem1' mem2' value H_combine_inj_2 H_mstore'_mem1 H_mstore'_mem2) as IHsize'_0.
+         rewrite IHsize'_0.
+
+         pose proof (eval_smemory_u_mem_1 (S n') size' offset offset' mem1 mem2 mem1' mem2' value H_mload''_mem1_mem2_0 H_mstore'_mem1 H_mstore'_mem2 ) as H_eval_smemory_u_mem_1.
+         rewrite H_eval_smemory_u_mem_1.
+         reflexivity.
+Qed.
+           
+  Lemma eval_smemory_u_mem_3:
+    forall size n offset offset' mem1 mem2 mem1' mem2' (value : word (n*8)) ,
+      mload' mem1 offset size = mload' mem2 offset size ->
+      mstore' mem1 value offset' = mem1' ->
+      mstore' mem2 value offset' = mem2' ->
+      mload' mem1' offset size = mload' mem2' offset size.
+  Proof.
+    unfold mload'.
+    intros size n offset offset' mem1 mem2 mem1' mem2' value.
+    intros H_mload'' H_mstore'_mem1 H_mstore'_mem2.
+    apply (eval_smemory_u_mem_2 size n (wordToN offset) offset' mem1 mem2 mem1' mem2' value H_mload'' H_mstore'_mem1 H_mstore'_mem2).
+  Qed.
+
+    Lemma eval_smemory_u_mem_4:
+    forall u offset size mem1 mem2 mem1' mem2',
+      mload' mem1 offset size = mload' mem2 offset size ->
+      update_memory' mem1 u = mem1' ->
+      update_memory' mem2 u = mem2' ->
+      mload' mem1' offset size = mload' mem2' offset size.
+    Proof.
+      intros u offset size mem1 mem2 mem1' mem2'.
+      intros H_mload' H_update_mem1 H_update_mem2.
+      destruct u as [uoffset uvalue|uoffset uvalue].
+      + simpl in *.
+        unfold mstore in *.
+        apply (eval_smemory_u_mem_3 size BytesInEVMWord offset (wordToN uoffset) mem1 mem2 mem1' mem2' uvalue H_mload' H_update_mem1 H_update_mem2).
+      + simpl in *.
+        unfold mstore in *.
+        apply (eval_smemory_u_mem_3 size 1 offset (wordToN uoffset) mem1 mem2 mem1' mem2' (split1_byte (uvalue: word ((S (pred BytesInEVMWord))*8))) H_mload' H_update_mem1 H_update_mem2).
+    Qed.
+        
+      
+  Lemma eval_smemory_u_mem_5:
+    forall updates offset size mem1 mem2 mem1' mem2',
+      mload' mem1 offset size = mload' mem2 offset size ->
+      update_memory mem1 updates = mem1' ->
+      update_memory mem2 updates = mem2' ->
+      mload' mem1' offset size = mload' mem2' offset size.
+  Proof.
+    induction updates as [|u updates' IHupdates'].
+    + intros offset size mem1 mem2 mem1' mem2'.
+      intros H_mload' H_update_mem1 H_update_mem2.
+      simpl in *.
+      rewrite <- H_update_mem1.
+      rewrite <- H_update_mem2.
+      apply H_mload'.
+    + intros offset size mem1 mem2 mem1' mem2'.
+      intros H_mload' H_update_mem1 H_update_mem2.
+      simpl in H_update_mem1.
+      simpl in H_update_mem2.
+      remember (update_memory mem1 updates') as mem1''.
+      remember (update_memory mem2 updates') as mem2''.
+      pose proof (IHupdates' offset size mem1 mem2 mem1'' mem2'' H_mload' (eq_sym Heqmem1'') (eq_sym Heqmem2'')) as H_mload'_0.      
+      apply (eval_smemory_u_mem_4 u offset size mem1'' mem2'' mem1' mem2' H_mload'_0 H_update_mem1 H_update_mem2).
+  Qed.
+
+  
+  Lemma update_out_of_slot_snd_2:
+    forall (smem1 smem2: smemory) (u: memory_update sstack_val) (maxidx : nat) (sb : sbindings) (instk_height : nat) (ops : stack_op_instr_map) (stk : list EVMWord) (mem : memory) (strg : storage) (exts : externals) (mem1 mem2 mem1' mem2' : memory) (offset size : EVMWord),    
+      length stk = instk_height ->    
+      valid_bindings instk_height maxidx sb ops ->
+      valid_smemory instk_height maxidx smem1 ->
+      valid_smemory instk_height maxidx smem2 ->
+      valid_smemory_update instk_height maxidx u ->
+      eval_smemory smem1 maxidx sb stk mem strg exts ops = Some mem1 ->
+      eval_smemory smem2 maxidx sb stk mem strg exts ops = Some mem2 ->
+      eval_smemory (u::smem1) maxidx sb stk mem strg exts ops = Some mem1' ->
+      eval_smemory (u::smem2) maxidx sb stk mem strg exts ops = Some mem2' ->
+      (mload' mem1 offset (wordToNat size)) = (mload' mem2 offset (wordToNat size)) ->
+      exists v,
+        (mload' mem1' offset (wordToNat size)) = v /\
+          (mload' mem2' offset (wordToNat size)) = v.
+  Proof.
+    intros smem1 smem2 u maidx sb instk_height ops stk mem strg exts mem1 mem2 mem1' mem2' offset size.
+    intros H_valid_len_stk H_valid_bs H_valid_smem1 H_valid_smem2 H_valid_u H_eval_smem1 H_eval_smem2 H_eval_u_smem1 H_eval_u_smem2 H_mload'.
+
+    unfold eval_smemory in H_eval_smem1.
+    destruct (map_option (instantiate_memory_update (fun sv : sstack_val => eval_sstack_val sv stk mem strg exts maidx sb ops)) smem1) as [updates1|] eqn:E_mo_updates1; try discriminate.
+    injection H_eval_smem1 as H_mem1.
+    
+    unfold eval_smemory in H_eval_smem2.
+    destruct (map_option (instantiate_memory_update (fun sv : sstack_val => eval_sstack_val sv stk mem strg exts maidx sb ops)) smem2) as [updates2|] eqn:E_mo_updates2; try discriminate.
+    injection H_eval_smem2 as H_mem2.
+    
+    unfold eval_smemory in H_eval_u_smem1.
+    destruct (map_option (instantiate_memory_update (fun sv : sstack_val => eval_sstack_val sv stk mem strg exts maidx sb ops)) (u::smem1)) as [u_updates1|] eqn:E_mo_u_updates1; try discriminate.
+    injection H_eval_u_smem1 as H_mem1'.
+
+    unfold eval_smemory in H_eval_u_smem2.
+    destruct (map_option (instantiate_memory_update (fun sv : sstack_val => eval_sstack_val sv stk mem strg exts maidx sb ops)) (u::smem2)) as [u_updates2|] eqn:E_mo_u_updates2; try discriminate.
+    injection H_eval_u_smem2 as H_mem2'.
+
+    pose proof (map_option_split (memory_update sstack_val) (memory_update EVMWord) (instantiate_memory_update (fun sv : sstack_val => eval_sstack_val sv stk mem strg exts maidx sb ops)) smem1 u_updates1 u E_mo_u_updates1) as E_mo_u_updates1_0.
+    destruct E_mo_u_updates1_0 as [uv1 [update1' [H_u_updates1 [H_uv1 H_updates1']]]].
+    rewrite E_mo_updates1 in H_updates1'.
+    injection H_updates1' as H_updates1'.
+
+    pose proof (map_option_split (memory_update sstack_val) (memory_update EVMWord) (instantiate_memory_update (fun sv : sstack_val => eval_sstack_val sv stk mem strg exts maidx sb ops)) smem2 u_updates2 u E_mo_u_updates2) as E_mo_u_updates2_0.
+    destruct E_mo_u_updates2_0 as [uv2 [update2' [H_u_updates2 [H_uv2 H_updates2']]]].
+    rewrite E_mo_updates2 in H_updates2'.
+    injection H_updates2' as H_updates2'.
+
+    rewrite H_uv1 in H_uv2.
+    injection H_uv2 as H_uv2.
+
+    rewrite <- H_uv2 in H_u_updates2.
+    
+    rewrite H_u_updates1 in H_mem1'.
+    simpl in H_mem1'.
+    
+    rewrite H_u_updates2 in H_mem2'.
+    simpl in H_mem2'.
+
+    rewrite <- H_updates1' in H_mem1'.
+    rewrite <- H_updates2' in H_mem2'.
+
+    rewrite H_mem1 in H_mem1'.
+    rewrite H_mem2 in H_mem2'.
+
+    
+    pose proof (eval_smemory_u_mem_4 uv1 offset (wordToNat size) mem1 mem2 mem1' mem2' H_mload' H_mem1' H_mem2') as H_mload'_0.
+    rewrite H_mload'_0.
+    exists (mload' mem2' offset (wordToNat size)).
+    split; try reflexivity.
+  Qed.
+
+         
+  Lemma remove_out_of_slot'_snd_1:
+    forall (min max: N) (smem smem_r: smemory) (maxidx : nat) (sb : sbindings) (instk_height : nat) (ops : stack_op_instr_map)
+           (stk : list EVMWord) (mem : memory) (strg : storage) (exts : externals) (mem1 mem1' : memory)
+           (offset size : EVMWord),    
+      length stk = instk_height ->    
+      valid_bindings instk_height maxidx sb ops ->
+      valid_smemory instk_height maxidx smem ->
+      eval_smemory smem maxidx sb stk mem strg exts ops = Some mem1 ->
+      eval_smemory smem_r maxidx sb stk mem strg exts ops = Some mem1' ->
+      ((wordToN offset) >= min)%N ->
+      (((wordToN offset)+(wordToN size)) <= max)%N ->
+      remove_out_of_slot' smem min max maxidx sb instk_height ops = smem_r ->
+      exists v,
+        (mload' mem1 offset (wordToNat size)) = v /\
+          (mload' mem1' offset (wordToNat size)) = v.
+  Proof.
+    intros min max.
+    induction smem as [|u smem'].
+    + intros smem_r maxidx sb instk_height ops stk mem strg exts mem1 mem1' offset size.
+      intros H_len_stk H_valid_sb H_valid_smem H_eval_smem H_eval_smem_r H_lb H_ub H_remove_out_of_slot'.
+      simpl in H_remove_out_of_slot'.
+      rewrite <- H_remove_out_of_slot' in H_eval_smem_r.
+      unfold eval_smemory in H_eval_smem.
+      simpl in H_eval_smem.
+      injection H_eval_smem as H_mem1.
+      unfold eval_smemory in H_eval_smem_r.
+      simpl in H_eval_smem_r.
+      injection H_eval_smem_r as H_mem1'.
+      rewrite <- H_mem1.
+      rewrite <- H_mem1'.
+      exists (mload' mem offset (wordToNat size)).
+      split; reflexivity.
+    + intros smem_r maxidx sb instk_height ops stk mem strg exts mem1 mem1' offset size.
+      intros H_len_stk H_valid_sb H_valid_smem H_eval_smem H_eval_smem_r H_lb H_ub H_remove_out_of_slot'.
+      unfold remove_out_of_slot' in H_remove_out_of_slot'.
+      fold remove_out_of_slot' in H_remove_out_of_slot'.
+      destruct (update_out_of_slot u min max maxidx sb instk_height ops) eqn:E_update_out_of_slot.
+      ++ simpl in H_valid_smem.
+         destruct H_valid_smem as [H_valid_u H_valid_smem'].
+         pose proof (eval_smemory_succ instk_height maxidx sb stk mem strg exts ops smem' (eq_sym H_len_stk) H_valid_smem' H_valid_sb) as H_eval_smem'.
+         destruct H_eval_smem' as [mem' H_eval_smem'].
+         pose proof (update_out_of_slot_snd_1 min max u smem' maxidx sb instk_height ops stk mem strg exts mem' mem1 offset size H_len_stk H_valid_sb H_valid_smem' H_valid_u H_eval_smem' H_eval_smem H_lb H_ub E_update_out_of_slot) as H_update_out_of_slot_snd_1.
+         destruct H_update_out_of_slot_snd_1 as [v [H_mload'_mem' H_mload_mem1]].
+         rewrite <- H_mload'_mem' in H_mload_mem1.
+         exists (mload' mem' offset (wordToNat size)).
+         rewrite H_mload_mem1.
+         split; try reflexivity.
+         pose proof (IHsmem' smem_r maxidx sb instk_height ops stk mem strg exts mem' mem1' offset size H_len_stk H_valid_sb H_valid_smem' H_eval_smem' H_eval_smem_r H_lb H_ub H_remove_out_of_slot') as IHsmem'_0.
+         destruct IHsmem'_0 as [v' [H_mload'_mem'_0 H_mload_mem1'_0]].
+         rewrite H_mload'_mem'_0.
+         rewrite H_mload_mem1'_0.
+         reflexivity.
+      ++ remember (remove_out_of_slot' smem' min max maxidx sb instk_height ops) as smem''.
+         rewrite <- H_remove_out_of_slot' in H_eval_smem_r.
+         simpl in H_valid_smem.
+         destruct H_valid_smem as [H_valid_u H_valid_smem'].
+         pose proof (remove_out_of_slot'_valid min max smem' smem'' maxidx sb instk_height ops H_valid_sb H_valid_smem' (eq_sym Heqsmem'')) as H_valid_smem''.
+         pose proof (eval_smemory_succ instk_height maxidx sb stk mem strg exts ops smem' (eq_sym H_len_stk) H_valid_smem' H_valid_sb) as H_eval_smem'.
+         destruct H_eval_smem' as [mem2 H_eval_smem'].
+         
+         pose proof (eval_smemory_succ instk_height maxidx sb stk mem strg exts ops smem'' (eq_sym H_len_stk) H_valid_smem'' H_valid_sb) as H_eval_smem''.
+         destruct H_eval_smem'' as [mem2' H_eval_smem''].
+         pose proof (IHsmem' smem'' maxidx sb instk_height ops stk mem strg exts mem2 mem2' offset size H_len_stk H_valid_sb H_valid_smem' H_eval_smem' H_eval_smem'' H_lb H_ub (eq_sym Heqsmem'' )) as IHsmem'_0.
+         destruct IHsmem'_0 as [v' [IHsmem'_0_1 IHsmem'_0_2]].
+         rewrite <- IHsmem'_0_2 in IHsmem'_0_1.
+         pose proof (update_out_of_slot_snd_2 smem' smem'' u maxidx sb instk_height ops stk mem strg exts mem2 mem2' mem1 mem1' offset size H_len_stk H_valid_sb H_valid_smem' H_valid_smem'' H_valid_u H_eval_smem' H_eval_smem'' H_eval_smem H_eval_smem_r IHsmem'_0_1) as H_update_out_of_slot_snd_2.
+         apply H_update_out_of_slot_snd_2.
+  Qed.
+             
+
+Lemma remove_out_of_slot'_snd:
+  forall (min max: N) (smem smem_r: smemory) (maxidx : nat) (sb : sbindings) (instk_height : nat) (ops : stack_op_instr_map)
+         (stk : list EVMWord) (mem : memory) (strg : storage) (exts : externals) (mem1 mem1' : memory)
+         (offset size : EVMWord),    
+    length stk = instk_height ->    
+    valid_bindings instk_height maxidx sb ops ->
+    valid_smemory instk_height maxidx smem ->
+    eval_smemory smem maxidx sb stk mem strg exts ops = Some mem1 ->
+    eval_smemory smem_r maxidx sb stk mem strg exts ops = Some mem1' ->
+    ((wordToN offset) >= min)%N ->
+    ( ((wordToN offset)+(wordToN size)) <= max)%N ->
+    remove_out_of_slot' smem min max maxidx sb instk_height ops = smem_r ->
+    exists v,
+      get_keccak256_exts exts (wordToNat size)
+        (mload' mem1 offset (wordToNat size)) = v /\
+        get_keccak256_exts exts (wordToNat size)
+          (mload' mem1' offset (wordToNat size)) = v.
+Proof.
+  intros min max smem smem_r maxidx sb instk_height ops stk mem strg exts mem1 mem1' offset size.
+  intros H_stk_len H_valid_sb H_valid_smem H_eval_smem H_eval_smem_r H_b1 H_b2 H_remove_out_of_slot'.
+  pose proof (remove_out_of_slot'_snd_1 min max smem smem_r maxidx sb instk_height ops stk mem strg exts mem1 mem1' offset size H_stk_len H_valid_sb H_valid_smem H_eval_smem H_eval_smem_r H_b1 H_b2 H_remove_out_of_slot') as H_snd_1.
+  destruct H_snd_1 as [v' [H_snd_1_0 H_snd_1_1]].
+  rewrite H_snd_1_0.
+  rewrite H_snd_1_1.
+  exists (get_keccak256_exts exts (wordToNat size) v').
+  split; reflexivity.
+Qed.
+  
+Lemma remove_out_of_slot_valid:
+    forall (soffset ssize : sstack_val) (smem smem': smemory) (maxidx : nat) (sb : sbindings) (instk_height : nat) (ops : stack_op_instr_map),
+      valid_sstack_value instk_height maxidx soffset ->
+      valid_sstack_value instk_height maxidx ssize ->
+      valid_bindings instk_height maxidx sb ops ->
+      valid_smemory instk_height maxidx smem ->
+      remove_out_of_slot smem soffset ssize maxidx sb instk_height ops = smem' ->
+      valid_smemory instk_height maxidx smem'.
+  Proof.
+    intros soffset ssize smem smem' maxidx sb instk_height ops.
+    intros H_valid_soffset H_valid_ssize H_valid_sb H_valid_smem H_remove_out_of_slot.
+    unfold remove_out_of_slot in H_remove_out_of_slot.
+    destruct (follow_in_smap soffset maxidx sb).
+     destruct f.
+      destruct smv.
+      destruct val.
+      destruct (follow_in_smap ssize maxidx sb).
+      destruct f.
+      destruct smv.
+      destruct val0.
+      pose proof (remove_out_of_slot'_valid (wordToN val) (wordToN val + wordToN val0) smem smem' maxidx sb instk_height ops H_valid_sb H_valid_smem H_remove_out_of_slot) as H_valid_smem'.
+      apply H_valid_smem'.
+
+      (* TODO somehow did not suceed to write ot with repeat, try again *)
+      rewrite <- H_remove_out_of_slot. apply H_valid_smem.
+      rewrite <- H_remove_out_of_slot. apply H_valid_smem.
+      rewrite <- H_remove_out_of_slot. apply H_valid_smem.
+      rewrite <- H_remove_out_of_slot. apply H_valid_smem.
+      rewrite <- H_remove_out_of_slot. apply H_valid_smem.
+      rewrite <- H_remove_out_of_slot. apply H_valid_smem.
+      rewrite <- H_remove_out_of_slot. apply H_valid_smem.
+      rewrite <- H_remove_out_of_slot. apply H_valid_smem.
+      rewrite <- H_remove_out_of_slot. apply H_valid_smem.
+      rewrite <- H_remove_out_of_slot. apply H_valid_smem.
+      rewrite <- H_remove_out_of_slot. apply H_valid_smem.
+      rewrite <- H_remove_out_of_slot. apply H_valid_smem.
+      rewrite <- H_remove_out_of_slot. apply H_valid_smem.
+      rewrite <- H_remove_out_of_slot. apply H_valid_smem.
+      rewrite <- H_remove_out_of_slot. apply H_valid_smem.
+      rewrite <- H_remove_out_of_slot. apply H_valid_smem.
+Qed.
+
+  Lemma remove_out_of_slot_snd:
+  forall (soffset ssize : sstack_val) (smem smem': smemory) (maxidx : nat) (sb : sbindings) (instk_height : nat) (ops : stack_op_instr_map),
+  valid_sstack_value instk_height maxidx soffset ->
+  valid_sstack_value instk_height maxidx ssize ->
+  valid_bindings instk_height maxidx sb ops ->
+  valid_smemory instk_height maxidx smem ->
+  remove_out_of_slot smem soffset ssize maxidx sb instk_height ops = smem' ->
+  forall (stk : list EVMWord) (mem : memory) (strg : storage) (exts : externals),
+    length stk = instk_height ->    
+    exists
+      (offset size : EVMWord) (mem1 mem1' : memory) (v : EVMWord),
+      eval_smemory smem maxidx sb stk mem strg exts ops = Some mem1 /\
+        eval_smemory smem' maxidx sb stk mem strg exts ops = Some mem1' /\
+        eval_sstack_val soffset stk mem strg exts maxidx sb ops = Some offset /\
+        eval_sstack_val ssize stk mem strg exts maxidx sb ops = Some size /\
+        get_keccak256_exts exts (wordToNat size)
+          (mload' mem1 offset (wordToNat size)) = v /\
+        get_keccak256_exts exts (wordToNat size)
+          (mload' mem1' offset (wordToNat size)) = v.
+  Proof.
+    intros soffset ssize smem smem' maxidx sb instk_height ops.
+    intros H_valid_soffset H_valid_ssize H_valid_sb H_valid_smem H_remove_out_of_slot.
+    intros stk mem strg exts H_stk_len.
+
+    pose proof (remove_out_of_slot_valid soffset ssize smem smem' maxidx sb instk_height ops H_valid_soffset H_valid_ssize H_valid_sb H_valid_smem H_remove_out_of_slot) as H_valid_smem'.
+
+    pose proof (eval_smemory_succ instk_height maxidx sb stk mem strg exts ops smem (eq_sym H_stk_len) H_valid_smem H_valid_sb) as H_eval_smem.
+    destruct H_eval_smem as [mem1 H_eval_smem].
+
+    pose proof (eval_smemory_succ instk_height maxidx sb stk mem strg exts ops smem' (eq_sym H_stk_len) H_valid_smem' H_valid_sb) as H_eval_smem'.
+    destruct H_eval_smem' as [mem1' H_eval_smem'].
+
+    pose proof (eval_sstack_val_succ sb instk_height soffset stk mem strg exts maxidx ops (eq_sym H_stk_len) H_valid_soffset H_valid_sb) as H_eval_soffset.
+    destruct H_eval_soffset as [soffset_v H_eval_soffset].
+
+    pose proof (eval_sstack_val_succ sb instk_height ssize stk mem strg exts maxidx ops (eq_sym H_stk_len) H_valid_ssize H_valid_sb) as H_eval_ssize.
+    destruct H_eval_ssize as [ssize_v H_eval_ssize].
+    
+
+    assert (H_aux: smem = smem' ->
+                     exists (offset size : EVMWord) (mem0 mem1'0 : memory) (v : EVMWord),
+    eval_smemory smem maxidx sb stk mem strg exts ops = Some mem0 /\
+    eval_smemory smem' maxidx sb stk mem strg exts ops = Some mem1'0 /\
+    eval_sstack_val soffset stk mem strg exts maxidx sb ops = Some offset /\
+    eval_sstack_val ssize stk mem strg exts maxidx sb ops = Some size /\
+    get_keccak256_exts exts (wordToNat size) (mload' mem0 offset (wordToNat size)) = v /\ get_keccak256_exts exts (wordToNat size) (mload' mem1'0 offset (wordToNat size)) = v
+           ).
+    (* proof of assert *)
+    intro H_smem_eq_smem'.
+
+    rewrite <- H_smem_eq_smem' in H_eval_smem'.
+    assert(H_mem1_eq_mem1' := H_eval_smem').
+    rewrite H_eval_smem in H_mem1_eq_mem1'.
+    injection H_mem1_eq_mem1' as H_mem1_eq_mem1'.
+    
+    
+    exists soffset_v. exists ssize_v. exists mem1. exists mem1'.
+    exists (get_keccak256_exts exts (wordToNat ssize_v) (mload' mem1 soffset_v (wordToNat ssize_v))).
+    rewrite <- H_smem_eq_smem'.
+    rewrite H_mem1_eq_mem1'.
+    split; try intuition.
+
+    unfold remove_out_of_slot in H_remove_out_of_slot.
+    destruct (follow_in_smap soffset maxidx sb) eqn:E_follow_soffset; try intuition.
+    destruct f.
+    destruct smv; try intuition.
+    destruct val; try intuition.
+    destruct (follow_in_smap ssize maxidx sb) eqn:E_follow_ssize; try intuition.
+    destruct f.
+    destruct smv; try intuition.
+    destruct val0; try intuition.
+
+
+    assert( H_eval_soffset' := H_eval_soffset).
+    unfold eval_sstack_val in H_eval_soffset.
+    unfold eval_sstack_val' in H_eval_soffset.
+    fold eval_sstack_val' in H_eval_soffset.
+    rewrite E_follow_soffset in H_eval_soffset.
+    injection H_eval_soffset as H_val_eq_soffset.
+
+    assert( H_eval_ssize' := H_eval_ssize).
+    unfold eval_sstack_val in H_eval_ssize.
+    unfold eval_sstack_val' in H_eval_ssize.
+    fold eval_sstack_val' in H_eval_ssize.
+    rewrite E_follow_ssize in H_eval_ssize.
+    injection H_eval_ssize as H_val0_eq_ssize.
+
+    
+    assert(H_l: (wordToN soffset_v >= wordToN val)%N).
+    (* proof of assert *)
+    rewrite H_val_eq_soffset.
+    apply N.le_ge.
+    apply N.le_refl.
+    (* end of proof of assert *)
+    
+    assert(H_u: (wordToN soffset_v + wordToN ssize_v  <= wordToN val + wordToN val0 )%N). 
+    (* proof of assert *)
+    rewrite H_val_eq_soffset.
+    rewrite H_val0_eq_ssize.
+    apply N.le_refl. 
+    (* end of proof of assert *)
+
+    pose proof (remove_out_of_slot'_snd (wordToN val) (wordToN val + wordToN val0) smem smem' maxidx sb instk_height ops stk mem strg exts mem1 mem1' soffset_v ssize_v H_stk_len H_valid_sb H_valid_smem H_eval_smem H_eval_smem' H_l H_u H_remove_out_of_slot) as H_remove_out_of_slot'_snd.
+    destruct H_remove_out_of_slot'_snd as [v H_remove_out_of_slot'_snd].
+
+    exists soffset_v. exists ssize_v. exists mem1. exists mem1'. exists v.
+    intuition.
+    
+  Qed.
+
   Lemma basic_sha3_cmp_snd:
     safe_sha3_cmp_ext_wrt_sstack_value_cmp basic_sha3_cmp.
   Proof.
-    Admitted.
+    unfold safe_sha3_cmp_ext_wrt_sstack_value_cmp.
+    intros d sstack_val_cmp H_safe_sstack_val_cmp.
+    unfold safe_sha3_cmp_ext_d.
+    intros d' H_d'_le_d.
+    unfold safe_sha3_cmp.
+    intros soffset1 ssize1 smem1 soffset2 ssize2 smem2 maxidx1 sb1 maxidx2 sb2 instk_height ops.
+    intros H_valid_soffset1 H_valid_ssize1 H_valid_soffset2 H_valid_ssize2 H_valid_sb1 H_valid_sb2 H_valid_smem1 H_valid_smem2.
+    intros H_basic_sha3_cmp.
+    intros stk mem strg exts H_stk_len.
+    unfold basic_sha3_cmp in H_basic_sha3_cmp.
+    destruct (sstack_val_cmp d' soffset1 soffset2 maxidx1 sb1 maxidx2 sb2 instk_height ops && sstack_val_cmp d' ssize1 ssize2 maxidx1 sb1 maxidx2 sb2 instk_height ops) eqn:H_eq_size_and_offset; try discriminate.
+    apply andb_prop in H_eq_size_and_offset as [H_eq_soffset H_eq_ssize].
+    remember (remove_out_of_slot smem1 soffset1 ssize1 maxidx1 sb1 instk_height ops) as smem1' eqn:H_smem1'.
+    remember (remove_out_of_slot smem2 soffset2 ssize2 maxidx2 sb2 instk_height ops) as smem2' eqn:H_smem2'.
 
+    pose proof (remove_out_of_slot_valid soffset1 ssize1 smem1 smem1' maxidx1 sb1 instk_height ops H_valid_soffset1 H_valid_ssize1 H_valid_sb1 H_valid_smem1 (eq_sym H_smem1')) as H_valid_smem1'.
+    
+    pose proof (remove_out_of_slot_snd soffset1 ssize1 smem1 smem1' maxidx1 sb1 instk_height ops H_valid_soffset1 H_valid_ssize1 H_valid_sb1 H_valid_smem1 (eq_sym H_smem1')) as H_out_of_slot_1_2.
+
+    pose proof (H_out_of_slot_1_2 stk mem strg exts H_stk_len) as H_out_of_slot_1_2.
+    destruct H_out_of_slot_1_2 as [ofsset1 [size1 [mem1 [mem1' [v1 [H_eval_smem1 [ H_eval_smem1' [ H_eval_soffset1 [ H_eval_ssize1 [H_sha3_mem1 H_sha3_mem1']]]]]]]]]].
+
+    pose proof (remove_out_of_slot_valid soffset2 ssize2 smem2 smem2' maxidx2 sb2 instk_height ops H_valid_soffset2 H_valid_ssize2 H_valid_sb2 H_valid_smem2 (eq_sym H_smem2')) as H_valid_smem2'.
+
+    pose proof (remove_out_of_slot_snd soffset2 ssize2 smem2 smem2' maxidx2 sb2 instk_height ops H_valid_soffset2 H_valid_ssize2 H_valid_sb2 H_valid_smem2 (eq_sym H_smem2')) as H_out_of_slot_2_2.
+    
+    pose proof (H_out_of_slot_2_2 stk mem strg exts H_stk_len) as H_out_of_slot_2_2.
+    destruct H_out_of_slot_2_2 as [ofsset2 [size2 [mem2 [mem2' [v2 [H_eval_smem2 [ H_eval_smem2' [ H_eval_soffset2 [ H_eval_ssize2 [H_sha3_mem2 H_sha3_mem2']]]]]]]]]].
+
+    pose proof (po_memory_cmp_snd) as H_po_memory_cmp_snd.
+    unfold safe_smemory_cmp_ext_wrt_sstack_value_cmp in H_po_memory_cmp_snd.
+    pose proof (H_po_memory_cmp_snd d sstack_val_cmp H_safe_sstack_val_cmp) as H_po_memory_cmp_snd.
+
+    unfold safe_smemory_cmp_ext_d in H_po_memory_cmp_snd.
+    pose proof (H_po_memory_cmp_snd d' H_d'_le_d) as H_po_memory_cmp_snd.
+    unfold safe_smemory_cmp in H_po_memory_cmp_snd.
+    pose proof (H_po_memory_cmp_snd smem1' smem2' maxidx1 sb1 maxidx2 sb2 instk_height ops H_valid_sb1 H_valid_sb2 H_valid_smem1' H_valid_smem2' H_basic_sha3_cmp stk mem strg exts H_stk_len) as H_po_memory_cmp_snd.
+    destruct H_po_memory_cmp_snd as [mem' [H_eval_smem1'_aux H_eval_smem2'_aux]].
+
+    rewrite H_eval_smem1'_aux in H_eval_smem1'.
+    injection H_eval_smem1' as H_mem'_eq_mem1'.
+
+    rewrite H_eval_smem2'_aux in H_eval_smem2'.
+    injection H_eval_smem2' as H_mem'_eq_mem2'.
+
+    rewrite H_mem'_eq_mem2' in H_mem'_eq_mem1'.
+
+    exists ofsset1. exists size1. exists mem1.
+    exists ofsset2. exists size2. exists mem2.
+    exists v1.
+
+
+    repeat split; try auto.
+
+
+    unfold safe_sstack_val_cmp_ext_1_d in H_safe_sstack_val_cmp.
+    pose proof (H_safe_sstack_val_cmp d' H_d'_le_d) as H_safe_sstack_val_cmp.
+    unfold safe_sstack_val_cmp in H_safe_sstack_val_cmp.
+
+    pose proof (H_safe_sstack_val_cmp soffset1 soffset2 maxidx1 sb1 maxidx2 sb2 instk_height ops H_valid_soffset1 H_valid_soffset2 H_valid_sb1 H_valid_sb2 H_eq_soffset stk mem strg exts H_stk_len) as H_safe_sstack_val_cmp_soffset.
+    destruct H_safe_sstack_val_cmp_soffset as [v_soffset [H_eval_soffset1' H_eval_soffset2']].
+
+    pose proof (H_safe_sstack_val_cmp ssize1 ssize2 maxidx1 sb1 maxidx2 sb2 instk_height ops H_valid_ssize1 H_valid_ssize2 H_valid_sb1 H_valid_sb2 H_eq_ssize stk mem strg exts H_stk_len) as H_safe_sstack_val_cmp_ssize.
+    destruct H_safe_sstack_val_cmp_ssize as [v_ssize [H_eval_ssize1' H_eval_ssize2']].
+
+    rewrite H_eval_soffset1 in H_eval_soffset1'.
+    injection H_eval_soffset1' as H_size1_eq_v_soffset.
+
+    rewrite H_eval_soffset2 in H_eval_soffset2'.
+    injection H_eval_soffset2' as H_size2_eq_v_soffset.
+
+    rewrite <- H_size1_eq_v_soffset in H_size2_eq_v_soffset.
+    
+    rewrite H_eval_ssize1 in H_eval_ssize1'.
+    injection H_eval_ssize1' as H_size1_eq_v_ssize.
+
+    rewrite H_eval_ssize2 in H_eval_ssize2'.
+    injection H_eval_ssize2' as H_size2_eq_v_ssize.
+
+    rewrite <- H_size1_eq_v_ssize in H_size2_eq_v_ssize.
+
+    rewrite H_sha3_mem2.
+
+    rewrite H_mem'_eq_mem1' in H_sha3_mem2'.
+    rewrite H_size2_eq_v_soffset in H_sha3_mem2'.
+    rewrite H_size2_eq_v_ssize in H_sha3_mem2'.
+
+    rewrite H_sha3_mem2' in H_sha3_mem1'.
+    apply H_sha3_mem1'.
+  Qed.
+  
 End SHA3CmpImplSoundness.
